## 题目：

$$
若f(x)=x^6-2\sqrt{2006}x^5-x^4+x^3-2\sqrt{2007}x^2+2x-\sqrt{2006} \\
则f（\sqrt{2006}+\sqrt{2007}）的值为？
$$

## 解答：

> 可以考虑把$\sqrt{2006}+\sqrt{2007}$转化为方程带入原式消元降次

$$
\begin{align}
& x=\sqrt{2006}+\sqrt{2007} \\
\Rightarrow & x-\sqrt{2006}=\sqrt{2007} \\
\Rightarrow & x^2-2\sqrt{2006}x+2006=2007\\
\Rightarrow & x^2-2\sqrt{2006}x-1=0 \\
同理，& x^2-2\sqrt{2007}x+1=0 \\\\
\therefore f(x)=&x^6-2\sqrt{2006}x^5-x^4+x^3-2\sqrt{2007}x^2+2x-\sqrt{2006} \\
=&x^4(x^2-2\sqrt{2006}x-1)+x(x^2-2\sqrt{2007}x+1)+x-\sqrt{2006} \\
=&x-\sqrt{2006} \\
=&\sqrt{2007} \\
=&3\sqrt{223}
\end{align}
$$

